Extend compartments to common libraries
Most of the changes are or appear to be straightforward. A number of new
subgoals are generated; these mostly require us to prove new instances
of block ownership or relate compartments across operations. These goals
should all be straightforward.

Because compartments are sometimes hidden in some top-level
formulations, some tactics need to change to their existential variants
in order to work.

In addition to these general remarks, it should be possible to extend
hint databases to discharge some of the new goals, just as other
similar subproofs are found by simple proof search.

common/Globalenvs.v
@@ -48,10 +48,10 @@ Set Implicit Arguments.
 
 (** Auxiliary function for initialization of global variables. *)
 
-Function store_zeros (m: mem) (b: block) (p: Z) (n: Z) {wf (Zwf 0) n}: option mem :=
+Function store_zeros (m: mem) (b: block) (p: Z) (n: Z) (cp: compartment) {wf (Zwf 0) n}: option mem :=
   if zle n 0 then Some m else
-    match Mem.store Mint8unsigned m b p Vzero with
-    | Some m' => store_zeros m' b (p + 1) (n - 1)
+    match Mem.store Mint8unsigned m b p Vzero cp with
+    | Some m' => store_zeros m' b (p + 1) (n - 1) cp
     | None => None
     end.
 Proof.
@@ -654,30 +654,31 @@ Section INITMEM.
 
 Variable ge: t.
 
-Definition store_init_data (m: mem) (b: block) (p: Z) (id: init_data) : option mem :=
+Definition store_init_data (m: mem) (b: block) (p: Z) (id: init_data) (cp: compartment) : option mem :=
   match id with
-  | Init_int8 n => Mem.store Mint8unsigned m b p (Vint n)
-  | Init_int16 n => Mem.store Mint16unsigned m b p (Vint n)
-  | Init_int32 n => Mem.store Mint32 m b p (Vint n)
-  | Init_int64 n => Mem.store Mint64 m b p (Vlong n)
-  | Init_float32 n => Mem.store Mfloat32 m b p (Vsingle n)
-  | Init_float64 n => Mem.store Mfloat64 m b p (Vfloat n)
+  | Init_int8 n => Mem.store Mint8unsigned m b p (Vint n) cp
+  | Init_int16 n => Mem.store Mint16unsigned m b p (Vint n) cp
+  | Init_int32 n => Mem.store Mint32 m b p (Vint n) cp
+  | Init_int64 n => Mem.store Mint64 m b p (Vlong n) cp
+  | Init_float32 n => Mem.store Mfloat32 m b p (Vsingle n) cp
+  | Init_float64 n => Mem.store Mfloat64 m b p (Vfloat n) cp
   | Init_addrof symb ofs =>
       match find_symbol ge symb with
       | None => None
-      | Some b' => Mem.store Mptr m b p (Vptr b' ofs)
+      | Some b' => Mem.store Mptr m b p (Vptr b' ofs) cp
       end
   | Init_space n => Some m
   end.
 
 Fixpoint store_init_data_list (m: mem) (b: block) (p: Z) (idl: list init_data)
+                              (cp : compartment)
                               {struct idl}: option mem :=
   match idl with
   | nil => Some m
   | id :: idl' =>
-      match store_init_data m b p id with
+      match store_init_data m b p id cp with
       | None => None
-      | Some m' => store_init_data_list m' b (p + init_data_size id) idl'
+      | Some m' => store_init_data_list m' b (p + init_data_size id) idl' cp
       end
   end.
 
@@ -690,17 +691,18 @@ Definition alloc_global (m: mem) (idg: ident * globdef F V): option mem :=
   match idg with
   | (id, Gfun f) =>
       let (m1, b) := Mem.alloc m (comp_of f) 0 1 in
-      Mem.drop_perm m1 b 0 1 Nonempty
+      Mem.drop_perm m1 b 0 1 Nonempty (comp_of f)
   | (id, Gvar v) =>
       let init := v.(gvar_init) in
+      let comp := v.(gvar_comp) in
       let sz := init_data_list_size init in
-      let (m1, b) := Mem.alloc m v.(gvar_comp) 0 sz in
-      match store_zeros m1 b 0 sz with
+      let (m1, b) := Mem.alloc m comp 0 sz in
+      match store_zeros m1 b 0 sz comp with
       | None => None
       | Some m2 =>
-          match store_init_data_list m2 b 0 init with
+          match store_init_data_list m2 b 0 init comp with
           | None => None
-          | Some m3 => Mem.drop_perm m3 b 0 sz (perm_globvar v)
+          | Some m3 => Mem.drop_perm m3 b 0 sz (perm_globvar v) comp
           end
       end
   end.
@@ -728,22 +730,22 @@ Qed.
 (** Next-block properties *)
 
 Remark store_zeros_nextblock:
-  forall m b p n m', store_zeros m b p n = Some m' -> Mem.nextblock m' = Mem.nextblock m.
+  forall m b p n cp m', store_zeros m b p n cp = Some m' -> Mem.nextblock m' = Mem.nextblock m.
 Proof.
-  intros until n. functional induction (store_zeros m b p n); intros.
+  intros until cp. functional induction (store_zeros m b p n cp); intros.
   inv H; auto.
   rewrite IHo; eauto with mem.
   congruence.
 Qed.
 
 Remark store_init_data_list_nextblock:
-  forall idl b m p m',
-  store_init_data_list m b p idl = Some m' ->
+  forall idl b m p cp m',
+  store_init_data_list m b p idl cp = Some m' ->
   Mem.nextblock m' = Mem.nextblock m.
 Proof.
   induction idl; simpl; intros until m'.
   intros. congruence.
-  caseEq (store_init_data m b p a); try congruence. intros.
+  caseEq (store_init_data m b p a cp); try congruence. intros.
   transitivity (Mem.nextblock m0). eauto.
   destruct a; simpl in H; try (eapply Mem.nextblock_store; eauto; fail).
   congruence.
@@ -787,24 +789,24 @@ Qed.
 (** Permissions *)
 
 Remark store_zeros_perm:
-  forall k prm b' q m b p n m',
-  store_zeros m b p n = Some m' ->
+  forall k prm b' q m b p n cp m',
+  store_zeros m b p n cp = Some m' ->
   (Mem.perm m b' q k prm <-> Mem.perm m' b' q k prm).
 Proof.
-  intros until n. functional induction (store_zeros m b p n); intros.
+  intros until cp. functional induction (store_zeros m b p n cp); intros.
   inv H; tauto.
   destruct (IHo _ H); intros. split; eauto with mem.
   congruence.
 Qed.
 
 Remark store_init_data_perm:
-  forall k prm b' q i b m p m',
-  store_init_data m b p i = Some m' ->
+  forall k prm b' q i cp b m p m',
+  store_init_data m b p i cp = Some m' ->
   (Mem.perm m b' q k prm <-> Mem.perm m' b' q k prm).
 Proof.
   intros.
   assert (forall chunk v,
-          Mem.store chunk m b p v = Some m' ->
+          Mem.store chunk m b p v cp = Some m' ->
           (Mem.perm m b' q k prm <-> Mem.perm m' b' q k prm)).
     intros; split; eauto with mem.
   destruct i; simpl in H; eauto.
@@ -813,8 +815,8 @@ Proof.
 Qed.
 
 Remark store_init_data_list_perm:
-  forall k prm b' q idl b m p m',
-  store_init_data_list m b p idl = Some m' ->
+  forall k prm b' q idl cp b m p m',
+  store_init_data_list m b p idl cp = Some m' ->
   (Mem.perm m b' q k prm <-> Mem.perm m' b' q k prm).
 Proof.
   induction idl as [ | i1 idl]; simpl; intros.
@@ -873,12 +875,12 @@ Qed.
 (** Data preservation properties *)
 
 Remark store_zeros_unchanged:
-  forall (P: block -> Z -> Prop) m b p n m',
-  store_zeros m b p n = Some m' ->
+  forall (P: block -> Z -> Prop) m b p n cp m',
+  store_zeros m b p n cp = Some m' ->
   (forall i, p <= i < p + n -> ~ P b i) ->
   Mem.unchanged_on P m m'.
 Proof.
-  intros until n. functional induction (store_zeros m b p n); intros.
+  intros until cp. functional induction (store_zeros m b p n cp); intros.
 - inv H; apply Mem.unchanged_on_refl.
 - apply Mem.unchanged_on_trans with m'.
 + eapply Mem.store_unchanged_on; eauto. simpl. intros. apply H0. omega.
@@ -887,8 +889,8 @@ Proof.
 Qed.
 
 Remark store_init_data_unchanged:
-  forall (P: block -> Z -> Prop) b i m p m',
-  store_init_data m b p i = Some m' ->
+  forall (P: block -> Z -> Prop) b i cp m p m',
+  store_init_data m b p i cp = Some m' ->
   (forall ofs, p <= ofs < p + init_data_size i -> ~ P b ofs) ->
   Mem.unchanged_on P m m'.
 Proof.
@@ -901,8 +903,8 @@ Proof.
 Qed.
 
 Remark store_init_data_list_unchanged:
-  forall (P: block -> Z -> Prop) b il m p m',
-  store_init_data_list m b p il = Some m' ->
+  forall (P: block -> Z -> Prop) b il cp m p m',
+  store_init_data_list m b p il cp = Some m' ->
   (forall ofs, p <= ofs -> ~ P b ofs) ->
   Mem.unchanged_on P m m'.
 Proof.
@@ -917,20 +919,23 @@ Qed.
 (** Properties related to [loadbytes] *)
 
 Definition readbytes_as_zero (m: mem) (b: block) (ofs len: Z) : Prop :=
-  forall p n,
+  forall p n cp,
   ofs <= p -> p + Z.of_nat n <= ofs + len ->
-  Mem.loadbytes m b p (Z.of_nat n) = Some (list_repeat n (Byte Byte.zero)).
+  Mem.loadbytes m b p (Z.of_nat n) cp = Some (list_repeat n (Byte Byte.zero)).
 
 Lemma store_zeros_loadbytes:
-  forall m b p n m',
-  store_zeros m b p n = Some m' ->
+  forall m b p n cp m',
+  store_zeros m b p n cp = Some m' ->
   readbytes_as_zero m' b p n.
 Proof.
-  intros until n; functional induction (store_zeros m b p n); red; intros.
+  intros until cp.
+  functional induction (store_zeros m b p n cp); red; intros.
 - destruct n0. simpl. apply Mem.loadbytes_empty. omega.
+  admit. (* RB: NOTE own_block assumption from loadbytes_empty *)
   rewrite Nat2Z.inj_succ in H1. omegaContradiction.
 - destruct (zeq p0 p).
   + subst p0. destruct n0. simpl. apply Mem.loadbytes_empty. omega.
+    admit. (* RB: NOTE own_block from loadbytes_empty *)
     rewrite Nat2Z.inj_succ in H1. rewrite Nat2Z.inj_succ.
     replace (Z.succ (Z.of_nat n0)) with (1 + Z.of_nat n0) by omega.
     change (list_repeat (S n0) (Byte Byte.zero))
@@ -942,11 +947,13 @@ Proof.
     replace (Byte Byte.zero :: nil) with (encode_val Mint8unsigned Vzero).
     change 1 with (size_chunk Mint8unsigned).
     eapply Mem.loadbytes_store_same; eauto.
+    admit. (* RB: NOTE: Seeming disagreement between assumption quantifiers  *)
     unfold encode_val; unfold encode_int; unfold rev_if_be; destruct Archi.big_endian; reflexivity.
     eapply IHo; eauto. omega. omega. omega. omega.
   + eapply IHo; eauto. omega. omega.
 - discriminate.
-Qed.
+(* Qed. *)
+Admitted.
 
 Definition bytes_of_init_data (i: init_data): list memval :=
   match i with
@@ -971,19 +978,19 @@ Proof.
 Qed.
 
 Lemma store_init_data_loadbytes:
-  forall m b p i m',
-  store_init_data m b p i = Some m' ->
+  forall m b p i cp m',
+  store_init_data m b p i cp = Some m' ->
   readbytes_as_zero m b p (init_data_size i) ->
-  Mem.loadbytes m' b p (init_data_size i) = Some (bytes_of_init_data i).
+  Mem.loadbytes m' b p (init_data_size i) cp = Some (bytes_of_init_data i).
 Proof.
-  intros; destruct i; simpl in H; try apply (Mem.loadbytes_store_same _ _ _ _ _ _ H).
+  intros; destruct i; simpl in H; try apply (Mem.loadbytes_store_same _ _ _ _ _ _ _ H).
 - inv H. simpl.
   assert (EQ: Z.of_nat (Z.to_nat z) = Z.max z 0).
   { destruct (zle 0 z). rewrite Z2Nat.id; xomega. destruct z; try discriminate. simpl. xomega. }
   rewrite <- EQ. apply H0. omega. simpl. omega.
 - rewrite init_data_size_addrof. simpl.
   destruct (find_symbol ge i) as [b'|]; try discriminate.
-  rewrite (Mem.loadbytes_store_same _ _ _ _ _ _ H).
+  rewrite (Mem.loadbytes_store_same _ _ _ _ _ _ _ H).
   unfold encode_val, Mptr; destruct Archi.ptr64; reflexivity.
 Qed.
 
@@ -994,13 +1001,14 @@ Fixpoint bytes_of_init_data_list (il: list init_data): list memval :=
   end.
 
 Lemma store_init_data_list_loadbytes:
-  forall b il m p m',
-  store_init_data_list m b p il = Some m' ->
+  forall b il m p cp m',
+  store_init_data_list m b p il cp = Some m' ->
   readbytes_as_zero m b p (init_data_list_size il) ->
-  Mem.loadbytes m' b p (init_data_list_size il) = Some (bytes_of_init_data_list il).
+  Mem.loadbytes m' b p (init_data_list_size il) cp = Some (bytes_of_init_data_list il).
 Proof.
   induction il as [ | i1 il]; simpl; intros.
 - apply Mem.loadbytes_empty. omega.
+  admit. (* RB: NOTE: own_block assumption from loadbytes_empty *)
 - generalize (init_data_size_pos i1) (init_data_list_size_pos il); intros P1 PL.
   destruct (store_init_data m b p i1) as [m1|] eqn:S; try discriminate.
   apply Mem.loadbytes_concat.
@@ -1018,15 +1026,16 @@ Proof.
   intros; omega.
   apply H0. omega. omega.
   auto. auto.
-Qed.
+(* Qed. *)
+Admitted.
 
 (** Properties related to [load] *)
 
-Definition read_as_zero (m: mem) (b: block) (ofs len: Z) : Prop :=
-  forall chunk p,
+Definition read_as_zero (m: mem) (b: block) (ofs len: Z) (cp: compartment) : Prop :=
+  forall chunk p cp,
   ofs <= p -> p + size_chunk chunk <= ofs + len ->
   (align_chunk chunk | p) ->
-  Mem.load chunk m b p =
+  Mem.load chunk m b p cp =
   Some (match chunk with
         | Mint8unsigned | Mint8signed | Mint16unsigned | Mint16signed | Mint32 => Vint Int.zero
         | Mint64 => Vlong Int64.zero
@@ -1036,20 +1045,20 @@ Definition read_as_zero (m: mem) (b: block) (ofs len: Z) : Prop :=
         end).
 
 Remark read_as_zero_unchanged:
-  forall (P: block -> Z -> Prop) m b ofs len m',
-  read_as_zero m b ofs len ->
+  forall (P: block -> Z -> Prop) m b ofs len cp m',
+  read_as_zero m b ofs len cp ->
   Mem.unchanged_on P m m' ->
   (forall i, ofs <= i < ofs + len -> P b i) ->
-  read_as_zero m' b ofs len.
+  read_as_zero m' b ofs len cp.
 Proof.
   intros; red; intros. eapply Mem.load_unchanged_on; eauto.
   intros; apply H1. omega.
 Qed.
 
 Lemma store_zeros_read_as_zero:
-  forall m b p n m',
-  store_zeros m b p n = Some m' ->
-  read_as_zero m' b p n.
+  forall m b p n cp m',
+  store_zeros m b p n cp = Some m' ->
+  read_as_zero m' b p n cp.
 Proof.
   intros; red; intros.
   transitivity (Some(decode_val chunk (list_repeat (size_chunk_nat chunk) (Byte Byte.zero)))).
@@ -1058,45 +1067,45 @@ Proof.
   f_equal. destruct chunk; unfold decode_val; unfold decode_int; unfold rev_if_be; destruct Archi.big_endian; reflexivity.
 Qed.
 
-Fixpoint load_store_init_data (m: mem) (b: block) (p: Z) (il: list init_data) {struct il} : Prop :=
+Fixpoint load_store_init_data (m: mem) (b: block) (p: Z) (il: list init_data) (cp: compartment) {struct il} : Prop :=
   match il with
   | nil => True
   | Init_int8 n :: il' =>
-      Mem.load Mint8unsigned m b p = Some(Vint(Int.zero_ext 8 n))
-      /\ load_store_init_data m b (p + 1) il'
+      Mem.load Mint8unsigned m b p cp = Some(Vint(Int.zero_ext 8 n))
+      /\ load_store_init_data m b (p + 1) il' cp
   | Init_int16 n :: il' =>
-      Mem.load Mint16unsigned m b p = Some(Vint(Int.zero_ext 16 n))
-      /\ load_store_init_data m b (p + 2) il'
+      Mem.load Mint16unsigned m b p cp = Some(Vint(Int.zero_ext 16 n))
+      /\ load_store_init_data m b (p + 2) il' cp
   | Init_int32 n :: il' =>
-      Mem.load Mint32 m b p = Some(Vint n)
-      /\ load_store_init_data m b (p + 4) il'
+      Mem.load Mint32 m b p cp = Some(Vint n)
+      /\ load_store_init_data m b (p + 4) il' cp
   | Init_int64 n :: il' =>
-      Mem.load Mint64 m b p = Some(Vlong n)
-      /\ load_store_init_data m b (p + 8) il'
+      Mem.load Mint64 m b p cp = Some(Vlong n)
+      /\ load_store_init_data m b (p + 8) il' cp
   | Init_float32 n :: il' =>
-      Mem.load Mfloat32 m b p = Some(Vsingle n)
-      /\ load_store_init_data m b (p + 4) il'
+      Mem.load Mfloat32 m b p cp = Some(Vsingle n)
+      /\ load_store_init_data m b (p + 4) il' cp
   | Init_float64 n :: il' =>
-      Mem.load Mfloat64 m b p = Some(Vfloat n)
-      /\ load_store_init_data m b (p + 8) il'
+      Mem.load Mfloat64 m b p cp = Some(Vfloat n)
+      /\ load_store_init_data m b (p + 8) il' cp
   | Init_addrof symb ofs :: il' =>
-      (exists b', find_symbol ge symb = Some b' /\ Mem.load Mptr m b p = Some(Vptr b' ofs))
-      /\ load_store_init_data m b (p + size_chunk Mptr) il'
+      (exists b', find_symbol ge symb = Some b' /\ Mem.load Mptr m b p cp = Some(Vptr b' ofs))
+      /\ load_store_init_data m b (p + size_chunk Mptr) il' cp
   | Init_space n :: il' =>
-      read_as_zero m b p n
-      /\ load_store_init_data m b (p + Z.max n 0) il'
+      read_as_zero m b p n cp
+      /\ load_store_init_data m b (p + Z.max n 0) il' cp
   end.
 
 Lemma store_init_data_list_charact:
-  forall b il m p m',
-  store_init_data_list m b p il = Some m' ->
-  read_as_zero m b p (init_data_list_size il) ->
-  load_store_init_data m' b p il.
+  forall b il m p cp m',
+  store_init_data_list m b p il cp = Some m' ->
+  read_as_zero m b p (init_data_list_size il) cp ->
+  load_store_init_data m' b p il cp.
 Proof.
-  assert (A: forall chunk v m b p m1 il m',
-    Mem.store chunk m b p v = Some m1 ->
-    store_init_data_list m1 b (p + size_chunk chunk) il = Some m' ->
-    Mem.load chunk m' b p = Some(Val.load_result chunk v)).
+  assert (A: forall chunk v m b p m1 il cp m',
+    Mem.store chunk m b p v cp = Some m1 ->
+    store_init_data_list m1 b (p + size_chunk chunk) il cp = Some m' ->
+    Mem.load chunk m' b p cp = Some(Val.load_result chunk v)).
   {
     intros.
     eapply Mem.load_unchanged_on with (P := fun b' ofs' => ofs' < p + size_chunk chunk).
@@ -1186,13 +1195,13 @@ Qed.
 
 Remark load_store_init_data_invariant:
   forall m m' b,
-  (forall chunk ofs, Mem.load chunk m' b ofs = Mem.load chunk m b ofs) ->
-  forall il p,
-  load_store_init_data m b p il -> load_store_init_data m' b p il.
+  (forall chunk ofs cp, Mem.load chunk m' b ofs cp = Mem.load chunk m b ofs cp) ->
+  forall il p cp,
+  load_store_init_data m b p il cp -> load_store_init_data m' b p il cp.
 Proof.
   induction il; intro p; simpl.
   auto.
-  rewrite ! H. destruct a; intuition. red; intros; rewrite H; auto.
+  intros. rewrite ! H. destruct a; intuition. red; intros; rewrite H; auto.
 Qed.
 
 Definition globals_initialized (g: t) (m: mem) :=
@@ -1200,14 +1209,14 @@ Definition globals_initialized (g: t) (m: mem) :=
   find_def g b = Some gd ->
   match gd with
   | Gfun f =>
-         Mem.perm m b 0 Cur Nonempty
+    Mem.perm m b 0 Cur Nonempty
       /\ (forall ofs k p, Mem.perm m b ofs k p -> ofs = 0 /\ p = Nonempty)
   | Gvar v =>
          Mem.range_perm m b 0 (init_data_list_size v.(gvar_init)) Cur (perm_globvar v)
       /\ (forall ofs k p, Mem.perm m b ofs k p ->
             0 <= ofs < init_data_list_size v.(gvar_init) /\ perm_order (perm_globvar v) p)
-      /\ (v.(gvar_volatile) = false -> load_store_init_data m b 0 v.(gvar_init))
-      /\ (v.(gvar_volatile) = false -> Mem.loadbytes m b 0 (init_data_list_size v.(gvar_init)) = Some (bytes_of_init_data_list v.(gvar_init)))
+      /\ (v.(gvar_volatile) = false -> load_store_init_data m b 0 v.(gvar_init) v.(gvar_comp))
+      /\ (v.(gvar_volatile) = false -> Mem.loadbytes m b 0 (init_data_list_size v.(gvar_init))v.(gvar_comp) = Some (bytes_of_init_data_list v.(gvar_init)))
   end.
 
 Lemma alloc_global_initialized:
@@ -1254,7 +1263,7 @@ Proof.
   eapply store_init_data_list_charact; eauto.
   eapply store_zeros_read_as_zero; eauto.
   intros NOTVOL.
-  transitivity (Mem.loadbytes m3 b 0 sz).
+  transitivity (Mem.loadbytes m3 b 0 sz v.(gvar_comp)).
   eapply Mem.loadbytes_drop; eauto. right; right; right.
   unfold perm_globvar. rewrite NOTVOL. destruct (gvar_readonly v); auto with mem.
   eapply store_init_data_list_loadbytes; eauto.
@@ -1358,9 +1367,9 @@ Theorem init_mem_characterization:
   /\ (forall ofs k p, Mem.perm m b ofs k p ->
         0 <= ofs < init_data_list_size gv.(gvar_init) /\ perm_order (perm_globvar gv) p)
   /\ (gv.(gvar_volatile) = false ->
-      load_store_init_data (globalenv p) m b 0 gv.(gvar_init))
+      load_store_init_data (globalenv p) m b 0 gv.(gvar_init) gv.(gvar_comp))
   /\ (gv.(gvar_volatile) = false ->
-      Mem.loadbytes m b 0 (init_data_list_size gv.(gvar_init)) = Some (bytes_of_init_data_list (globalenv p) gv.(gvar_init))).
+      Mem.loadbytes m b 0 (init_data_list_size gv.(gvar_init)) gv.(gvar_comp) = Some (bytes_of_init_data_list (globalenv p) gv.(gvar_init))).
 Proof.
   intros. rewrite find_var_info_iff in H.
   exploit init_mem_characterization_gen; eauto.
@@ -1386,23 +1395,23 @@ Variable thr: block.
 Hypothesis symb_inject: forall id b, find_symbol ge id = Some b -> Plt b thr.
 
 Lemma store_zeros_neutral:
-  forall m b p n m',
+  forall m b p n cp m',
   Mem.inject_neutral thr m ->
   Plt b thr ->
-  store_zeros m b p n = Some m' ->
+  store_zeros m b p n cp = Some m' ->
   Mem.inject_neutral thr m'.
 Proof.
-  intros until n. functional induction (store_zeros m b p n); intros.
+  intros until cp. functional induction (store_zeros m b p n cp); intros.
   inv H1; auto.
   apply IHo; auto. eapply Mem.store_inject_neutral; eauto. constructor.
   inv H1.
 Qed.
 
 Lemma store_init_data_neutral:
-  forall m b p id m',
+  forall m b p id cp m',
   Mem.inject_neutral thr m ->
   Plt b thr ->
-  store_init_data ge m b p id = Some m' ->
+  store_init_data ge m b p id cp = Some m' ->
   Mem.inject_neutral thr m'.
 Proof.
   intros.
@@ -1415,10 +1424,10 @@ Proof.
 Qed.
 
 Lemma store_init_data_list_neutral:
-  forall b idl m p m',
+  forall b idl m p cp m',
   Mem.inject_neutral thr m ->
   Plt b thr ->
-  store_init_data_list ge m b p idl = Some m' ->
+  store_init_data_list ge m b p idl cp = Some m' ->
   Mem.inject_neutral thr m'.
 Proof.
   induction idl; simpl; intros.
@@ -1519,16 +1528,16 @@ Section INITMEM_INVERSION.
 Variable ge: t.
 
 Lemma store_init_data_aligned:
-  forall m b p i m',
-  store_init_data ge m b p i = Some m' ->
+  forall m b p i cp m',
+  store_init_data ge m b p i cp = Some m' ->
   (init_data_alignment i | p).
 Proof.
   intros.
   assert (DFL: forall chunk v,
-    Mem.store chunk m b p v = Some m' ->
+    Mem.store chunk m b p v cp = Some m' ->
     align_chunk chunk = init_data_alignment i ->
     (init_data_alignment i | p)).
-  { intros. apply Mem.store_valid_access_3 in H0. destruct H0. congruence. }
+  { intros. apply Mem.store_valid_access_3 in H0. destruct H0 as [? [? ?]]. congruence. }
   destruct i; simpl in H; eauto.
   simpl. apply Z.divide_1_l.
   destruct (find_symbol ge i); try discriminate. eapply DFL. eassumption.
@@ -1536,8 +1545,8 @@ Proof.
 Qed.
 
 Lemma store_init_data_list_aligned:
-  forall b il m p m',
-  store_init_data_list ge m b p il = Some m' ->
+  forall b il m p cp m',
+  store_init_data_list ge m b p il cp = Some m' ->
   init_data_list_aligned p il.
 Proof.
   induction il as [ | i1 il]; simpl; intros.
@@ -1547,8 +1556,8 @@ Proof.
 Qed.
 
 Lemma store_init_data_list_free_idents:
-  forall b i o il m p m',
-  store_init_data_list ge m b p il = Some m' ->
+  forall b i o il m p cp m',
+  store_init_data_list ge m b p il cp = Some m' ->
   In (Init_addrof i o) il ->
   exists b', find_symbol ge i = Some b'.
 Proof.
@@ -1589,32 +1598,37 @@ Section INITMEM_EXISTS.
 Variable ge: t.
 
 Lemma store_zeros_exists:
-  forall m b p n,
-  Mem.range_perm m b p (p + n) Cur Writable ->
-  exists m', store_zeros m b p n = Some m'.
+  forall m b p n cp,
+    Mem.range_perm m b p (p + n) Cur Writable ->
+    Mem.own_block m b cp ->
+  exists m', store_zeros m b p n cp = Some m'.
 Proof.
-  intros until n. functional induction (store_zeros m b p n); intros PERM.
+  intros until cp. functional induction (store_zeros m b p n cp); intros PERM.
 - exists m; auto.
-- apply IHo. red; intros. eapply Mem.perm_store_1; eauto. apply PERM. omega.
-- destruct (Mem.valid_access_store m Mint8unsigned b p Vzero) as (m' & STORE).
+- intros. apply IHo. red; intros. eapply Mem.perm_store_1; eauto. apply PERM. omega.
+  admit. (* RB: NOTE: New own_block subgoal *)
+- destruct (Mem.valid_access_store m Mint8unsigned b p cp Vzero) as (m' & STORE).
   split. red; intros. apply Mem.perm_cur. apply PERM. simpl in H. omega.
+  split. admit. (* RB: NOTE: new own_block subgoal *)
   simpl. apply Z.divide_1_l.
   congruence.
-Qed.
+(* Qed. *)
+Admitted.
 
 Lemma store_init_data_exists:
-  forall m b p i,
+  forall m b p i cp,
   Mem.range_perm m b p (p + init_data_size i) Cur Writable ->
+  forall OWN : Mem.own_block m b cp,
   (init_data_alignment i | p) ->
   (forall id ofs, i = Init_addrof id ofs -> exists b, find_symbol ge id = Some b) ->
-  exists m', store_init_data ge m b p i = Some m'.
+  exists m', store_init_data ge m b p i cp = Some m'.
 Proof.
   intros.
   assert (DFL: forall chunk v,
           init_data_size i = size_chunk chunk ->
           init_data_alignment i = align_chunk chunk ->
-          exists m', Mem.store chunk m b p v = Some m').
-  { intros. destruct (Mem.valid_access_store m chunk b p v) as (m' & STORE).
+          exists m', Mem.store chunk m b p v cp = Some m').
+  { intros. destruct (Mem.valid_access_store m chunk b p cp v) as (m' & STORE).
     split. rewrite <- H2; auto. rewrite <- H3; auto.
     exists m'; auto. }
   destruct i; eauto.
@@ -1625,21 +1639,24 @@ Proof.
 Qed.
 
 Lemma store_init_data_list_exists:
-  forall b il m p,
+  forall b il m p cp,
   Mem.range_perm m b p (p + init_data_list_size il) Cur Writable ->
+  forall OWN : Mem.own_block m b cp,
   init_data_list_aligned p il ->
   (forall id ofs, In (Init_addrof id ofs) il -> exists b, find_symbol ge id = Some b) ->
-  exists m', store_init_data_list ge m b p il = Some m'.
+  exists m', store_init_data_list ge m b p il cp = Some m'.
 Proof.
   induction il as [ | i1 il ]; simpl; intros.
 - exists m; auto.
 - destruct H0.
-  destruct (@store_init_data_exists m b p i1) as (m1 & S1); eauto.
+  destruct (@store_init_data_exists m b p i1 cp) as (m1 & S1); eauto.
   red; intros. apply H. generalize (init_data_list_size_pos il); omega.
   rewrite S1.
   apply IHil; eauto.
   red; intros. erewrite <- store_init_data_perm by eauto. apply H. generalize (init_data_size_pos i1); omega.
-Qed.
+  admit. (* RB: NOTE: New own_block subgoal. *)
+(* Qed. *)
+Admitted.
 
 Lemma alloc_global_exists:
   forall m idg,
@@ -1653,26 +1670,31 @@ Lemma alloc_global_exists:
 Proof.
   intros m [id [f|v]]; intros; simpl.
 - destruct (Mem.alloc m _ 0 1) as [m1 b] eqn:ALLOC.
-  destruct (Mem.range_perm_drop_2 m1 b 0 1 Nonempty) as [m2 DROP].
+  destruct (Mem.range_perm_drop_2 m1 b 0 1 (comp_of f) Nonempty) as [m2 DROP].
   red; intros; eapply Mem.perm_alloc_2; eauto.
+  admit. (* RB: NOTE: New own_block subgoal *)
   exists m2; auto.
 - destruct H as [P Q].
   set (sz := init_data_list_size (gvar_init v)).
   destruct (Mem.alloc m _ 0 sz) as [m1 b] eqn:ALLOC.
   assert (P1: Mem.range_perm m1 b 0 sz Cur Freeable) by (red; intros; eapply Mem.perm_alloc_2; eauto).
-  destruct (@store_zeros_exists m1 b 0 sz) as [m2 ZEROS].
+  destruct (@store_zeros_exists m1 b 0 sz (gvar_comp v)) as [m2 ZEROS].
   red; intros. apply Mem.perm_implies with Freeable; auto with mem.
+  admit. (* RB: NOTE: New own_block subgoal *)
   rewrite ZEROS.
   assert (P2: Mem.range_perm m2 b 0 sz Cur Freeable).
   { red; intros. erewrite <- store_zeros_perm by eauto. eauto. }
-  destruct (@store_init_data_list_exists b (gvar_init v) m2 0) as [m3 STORE]; auto.
+  destruct (@store_init_data_list_exists b (gvar_init v) m2 0 (gvar_comp v)) as [m3 STORE]; auto.
   red; intros. apply Mem.perm_implies with Freeable; auto with mem.
+  admit. (* RB: NOTE: New own_block subgoal *)
   rewrite STORE.
   assert (P3: Mem.range_perm m3 b 0 sz Cur Freeable).
   { red; intros. erewrite <- store_init_data_list_perm by eauto. eauto. }
-  destruct (Mem.range_perm_drop_2 m3 b 0 sz (perm_globvar v)) as [m4 DROP]; auto.
+  destruct (Mem.range_perm_drop_2 m3 b 0 sz (gvar_comp v) (perm_globvar v)) as [m4 DROP]; auto.
+  admit. (* RB: NOTE: New own_block subgoal *)
   exists m4; auto.
-Qed.
+(* Qed. *)
+Admitted.
 
 End INITMEM_EXISTS.
 
@@ -1759,7 +1781,8 @@ Qed.
 Theorem find_def_match_2:
   forall b, option_rel (match_globdef match_fundef match_varinfo ctx)
                        (find_def (globalenv p) b) (find_def (globalenv tp) b).
-Proof (mge_defs globalenvs_match).
+(* Proof (mge_defs globalenvs_match). *)
+Admitted. (* RB: NOTE: open own_block goals *)
 
 Theorem find_def_match:
   forall b g,
@@ -1829,14 +1852,14 @@ Proof.
 Qed.
 
 Lemma store_init_data_list_match:
-  forall idl m b ofs m',
-  store_init_data_list (globalenv p) m b ofs idl = Some m' ->
-  store_init_data_list (globalenv tp) m b ofs idl = Some m'.
+  forall idl m b ofs cp m',
+  store_init_data_list (globalenv p) m b ofs idl cp = Some m' ->
+  store_init_data_list (globalenv tp) m b ofs idl cp = Some m'.
 Proof.
   induction idl; simpl; intros.
 - auto.
 - destruct (store_init_data (globalenv p) m b ofs a) as [m1|] eqn:S; try discriminate.
-  assert (X: store_init_data (globalenv tp) m b ofs a = Some m1).
+  assert (X: store_init_data (globalenv tp) m b ofs a cp = Some m1).
   { destruct a; auto. simpl; rewrite find_symbol_match; auto. }
   rewrite X. auto.
 Qed.
@@ -1854,6 +1877,7 @@ Proof.
   { destruct a1 as [id1 g1]; destruct b1 as [id2 g2]; destruct H; simpl in *.
     subst id2. inv H2.
   - erewrite <- match_fundef_comp; eauto.
+    erewrite <- match_fundef_comp; eauto.
   - inv H; simpl in *. simpl in Heqo.
     set (sz := init_data_list_size init) in *.
     destruct (Mem.alloc m _ 0 sz) as [m2 b] eqn:?.
